×’×œ×¢×“ ×‘×¨× ×¢ ×ª.×–. 203627310
# ××"×Ÿ 11
## 1
Prove: 
AÎ”BâŠ†D âˆ§ BÎ”CâŠ†D â†’ AÎ”CâŠ†D
<div class="line"></div>
Since (Xâ†’Z) âˆ§ (Yâ†’Z) â‰¡ (Xâˆ¨Y)â†’Z, also:
(AÎ”BâŠ†D âˆ§ BÎ”CâŠ†D) â‰¡ (AÎ”B âˆª BÎ”C) âŠ† D. Proof:
<box>
(Xâ†’Z) âˆ§ (Yâ†’Z)
Zâˆ¨Â¬X âˆ§ Zâˆ¨Â¬Y
Zâˆ¨Â¬(Xâˆ¨Y)
(Xâˆ¨Y) â†’ Z

AÎ”BâŠ†D âˆ§ BÎ”CâŠ†D
(xâˆˆ(AÎ”B) â†’ xâˆˆD) âˆ§ (xâˆˆ(BÎ”C) â†’ xâˆˆD)
xâˆˆ(AÎ”B âˆª BÎ”C) â†’ xâˆˆD
(AÎ”B âˆª BÎ”C) âŠ† D
Therefore:
(AÎ”BâŠ†D âˆ§ BÎ”CâŠ†D) â‰¡ (AÎ”B âˆª BÎ”C) âŠ† D // (1)
</box>
<line>
I'll prove that AÎ”C âŠ† (AÎ”B âˆª BÎ”C).
<thin>
Expanding (AÎ”B âˆª BÎ”C):
(<oline>B</oline>âˆ©A) âˆª (<oline>B</oline>âˆ©C) âˆª (Bâˆ©<oline>A</oline>) âˆª (Bâˆ©<oline>C</oline>)
[<oline>B</oline>n(AuC)] âˆª [Bn(<oline>A</oline>u<oline>C</oline>)]
__(AÎ”B âˆª BÎ”C) â‰¡ [<oline>B</oline>n(AuC)] âˆª [Bn(<oline>A</oline>u<oline>C</oline>)]__ // (2)


Expanding AÎ”C:
(An<oline>C</oline>) u (<oline>A</oline>nC)
(AâˆªC) n (<oline>A</oline>u<oline>C</oline>)
__AÎ”C â‰¡ (AâˆªC) n (<oline>A</oline>u<oline>C</oline>)__ // (3)

<thin>
Define: 
P = B; Q = (AuC); R = (<oline>A</oline>u<oline>C</oline>)
So proving Qâˆ§R â†’ (Â¬Pâˆ¨Q âˆ¨ Pâˆ§R),
will prove that AÎ”C âŠ† (AÎ”B âˆª BÎ”C)
<thin>
Proving Qâˆ§R â†’ (Â¬Pâˆ¨Q âˆ¨ Pâˆ§R) is always true:
Premise: (Qâˆ§R); Conclusion: (Â¬Pâˆ¨Q âˆ¨ Pâˆ§R).
Premise â†’ Conclusion is always true if the following holds:
Whenever the Premise is true, also the Conclusion is true.
Assuming that Premise is true:
Qâˆ§R â‰¡ ğš» âŸ¹ 
Qâ‰¡ğš» âˆ§ Râ‰¡ğš»
Using that \in the Conclusion:
(Â¬Pâˆ¨Q âˆ¨ Pâˆ§R) â‰¡ (Â¬Pâˆ¨ğš» âˆ¨ Pâˆ§ğš») â‰¡ Â¬Pâˆ¨P â‰¡ ğš»
Therefore the conclusion is dependent upon the premise, therefore 
__Qâˆ§R â†’ (Â¬Pâˆ¨Q âˆ¨ Pâˆ§R) â‰¡ ğš»__ // (4)
<thin>
P, Q \and R are placeholders (defined above), so I'll use their "real" values:
Qâˆ§R â†’ (Â¬Pâˆ¨Q âˆ¨ Pâˆ§R) â‰¡
(AâˆªC)âˆ©(<oline>A</oline>u<oline>C</oline>) â†’ [<oline>B</oline>n(AuC)] âˆª [Bn(<oline>A</oline>u<oline>C</oline>)]
// Using (3):
AÎ”C âŠ† [<oline>B</oline>n(AuC)] âˆª [Bn(<oline>A</oline>u<oline>C</oline>)]
// Using (2):
__AÎ”C âŠ† (AÎ”B âˆª BÎ”C)__ // (5)
<thin>
Since it's given that:
AÎ”BâŠ†D âˆ§ BÎ”CâŠ†D
Using (1), it's equivalent to:
(AÎ”B âˆª BÎ”C) âŠ† D
And because of (5), we know that 
AÎ”C âŠ† (AÎ”B âˆª BÎ”C)
Together with the transience of âŠ†, // XâŠ†Y \and YâŠ†Z => XâŠ†Z
__AÎ”BâŠ†D âˆ§ BÎ”CâŠ†D â†’ AÎ”CâŠ†D__